write some invariant code

concurrency/hack-hash-table/ResourceStateMachine.i.dfy
@@ -2,6 +2,7 @@ include "HTResource.i.dfy"
 
 module ResourceStateMachine {
   import opened KeyValueType
+  import opened Options
 
   import HT = HTResource
   import MapIfc
@@ -20,25 +21,139 @@ module ResourceStateMachine {
 
   predicate NewTicket(s: Variables, s': Variables, id: int, input: MapIfc.Input)
   {
-    s' == HT.add(s, HT.input_ticket(input))
+    s' == HT.add(s, HT.input_ticket(id, input))
   }
 
-  predicate ConsumeStub(s: Variables, s': Variables, id: int, output: MapIfc.Input)
+  predicate ConsumeStub(s: Variables, s': Variables, id: int, output: MapIfc.Output)
   {
-    s == HT.add(s', HT.output_stub(output))
+    s == HT.add(s', HT.output_stub(id, output))
   }
 
   ////// Invariant
 
-  predicate Complete(s: Variables)
+  predicate Complete(table: seq<Option<HT.Info>>)
   {
-    && (forall i | 0 <= i < |s.table| :: s.table[i].Some?)
+    && (forall i | 0 <= i < |table| :: table[i].Some?)
+  }
+
+  function adjust(i: int, root: int) : int
+  {
+    if i < root then HT.FixedSize() + i else i
+  }
+
+  // Keys are unique, although we don't count entries being removed
+  predicate KeysUnique(table: seq<Option<HT.Info>>)
+  requires Complete(table)
+  {
+    forall i, j | 0 <= i < |table| && 0 <= j < |table| && i != j
+      && table[i].value.entry.Full? && table[j].value.entry.Full?
+      && !table[i].value.state.RemoveTidying? && !table[j].value.state.RemoveTidying?
+        :: table[i].value.entry.kv.key != table[j].value.entry.kv.key
+  }
+
+  // If there's an entry in slot `i` with hash `h`, then
+  // you must be able to get from `h` to `i` (possibly wrapping around)
+  // with passing a free space.
+  predicate ContiguousToEntry(table: seq<Option<HT.Info>>, i: int)
+  requires Complete(table)
+  requires 0 <= i < |table|
+  {
+    table[i].value.entry.Full? ==> (
+      var h := HT.hash(table[i].value.entry.kv.key) as int;
+      && (h <= i ==> (forall j | h <= j <= i :: table[j].value.entry.Full?))
+      && (h > i ==>
+        && h < |table|
+        && (forall j | 0 <= j <= i :: table[j].value.entry.Full?)
+        && (forall j | h <= j < |table| :: table[j].value.entry.Full?)
+      )
+    )
+  }
+
+  // 'Robin Hood' order
+  // It's not enough to say that hash(entry[i]) <= hash(entry[i+1])
+  // because of wraparound. We do a cyclic comparison 'rooted' at an
+  // arbitrary empty element, given by e.
+  predicate ValidHashNeighbors(table: seq<Option<HT.Info>>, e: int, j: int)
+  requires Complete(table)
+  requires 0 <= e < |table|
+  requires 0 <= j < |table|
+  {
+    var k := (if j+1 < |table| then j+1 else 0);
+    (table[e].value.entry.Empty? && table[j].value.entry.Full? && table[k].value.entry.Full? ==> (
+      var hj := HT.hash(table[j].value.entry.kv.key) as int;
+      var hk := HT.hash(table[k].value.entry.kv.key) as int;
+      adjust(hj, e) <= adjust(hk, e)
+    ))
+  }
+
+  predicate ExistsEmptyEntry(table: seq<Option<HT.Info>>)
+  {
+    exists i :: 0 <= i < |table| && table[i].Some? && table[i].value.entry.Empty?
   }
 
   predicate Inv(s: Variables)
   {
     && s.R?
-    && Complete(s)
-    && 
+    && Complete(s.table)
+    && ExistsEmptyEntry(s.table)
+    && KeysUnique(s.table)
+    && (forall i | 0 <= i < |s.table| :: ContiguousToEntry(s.table, i))
+    && (forall e, j | 0 <= e < |s.table| && 0 <= j < |s.table|
+        :: ValidHashNeighbors(s.table, e, j))
   }
+
+  lemma ProcessInsertTicket_PreservesInv(s: Variables, s': Variables, insert_ticket: HT.Ticket)
+  requires Inv(s)
+  requires HT.ProcessInsertTicket(s, s', insert_ticket)
+  ensures Inv(s')
+  {
+    assert forall i | 0 <= i < |s'.table| :: s'.table[i].value.entry == s.table[i].value.entry;
+    forall i | 0 <= i < |s'.table|
+    ensures ContiguousToEntry(s'.table, i)
+    {
+      assert ContiguousToEntry(s.table, i);
+    }
+    forall e, j | 0 <= e < |s'.table| && 0 <= j < |s'.table|
+    ensures ValidHashNeighbors(s'.table, e, j)
+    {
+      assert ValidHashNeighbors(s.table, e, j);
+    }
+  }
+
+  lemma InsertSkip_PreservesInv(s: Variables, s': Variables, pos: nat)
+  requires Inv(s)
+  requires HT.InsertSkip(s, s', pos)
+  ensures Inv(s')
+  {
+    assert forall i | 0 <= i < |s'.table| :: s'.table[i].value.entry == s.table[i].value.entry;
+    forall i | 0 <= i < |s'.table|
+    ensures ContiguousToEntry(s'.table, i)
+    {
+      assert ContiguousToEntry(s.table, i);
+    }
+    forall e, j | 0 <= e < |s'.table| && 0 <= j < |s'.table|
+    ensures ValidHashNeighbors(s'.table, e, j)
+    {
+      assert ValidHashNeighbors(s.table, e, j);
+    }
+  }
+
+  lemma InsertSwap_PreservesInv(s: Variables, s': Variables, pos: nat)
+  requires Inv(s)
+  requires HT.InsertSwap(s, s', pos)
+  ensures Inv(s')
+  {
+    assert forall i | 0 <= i < |s'.table| :: s.table[i].value.entry.Empty? ==> s'.table[i].value.entry.Empty?;
+    forall i | 0 <= i < |s'.table|
+    ensures ContiguousToEntry(s'.table, i)
+    {
+      assert ContiguousToEntry(s.table, i);
+    }
+    forall e, j | 0 <= e < |s'.table| && 0 <= j < |s'.table|
+    ensures ValidHashNeighbors(s'.table, e, j)
+    {
+      assert ValidHashNeighbors(s.table, e, j);
+    }
+  }
+
 }
